Show more casts in PHOAS printing, sometimes (#1450)
* Show more casts in PHOAS printing

Rather than trying to be clever about which casts to print, we instead
always print all casts when displaying PHOAS.  This can be overridden
via typeclass instances by leaving around other values for
`PHOAS.with_casts` (boolean controling the previous default) and
`PHOAS.with_all_casts` (boolean controlling the new default, overriding
`PHOAS.with_casts`).

* Only show extra casts sometimes

src/Stringification/Language.v
@@ -51,6 +51,21 @@ Module Compilers.
   Local Notation tZ := (base.type.type_base base.type.Z).
 
   Module Export Options.
+    Module PHOAS.
+      (** Print casts in PHOAS? *)
+      Class with_casts := with_castsv : bool.
+      #[global] Typeclasses Opaque with_casts.
+
+      (** Print all casts in PHOAS? *)
+      Class with_all_casts := with_all_castsv : bool.
+      #[global] Typeclasses Opaque with_all_casts.
+
+      Definition default_with_casts : with_casts := true.
+      Definition default_with_all_casts : with_all_casts := false.
+    End PHOAS.
+    #[global] Typeclasses Opaque PHOAS.with_casts PHOAS.with_all_casts.
+    #[global] Existing Instances PHOAS.default_with_casts PHOAS.default_with_all_casts.
+
     (** How to relax zranges *)
     Class relax_zrange_opt := relax_zrange : zrange -> zrange.
 #[global]
@@ -592,9 +607,10 @@ Module Compilers.
         Local Notation show_lvl_preop idc := (lookup_show_lvl_preop conservative_preop_precedence_table (ident_to_op_string idc)).
         Local Notation show_lvl_postop idc := (lookup_show_lvl_postop conservative_postop_precedence_table (ident_to_op_string idc)).
 
-        Definition show_ident_lvl (with_casts : bool) {t} (idc : ident.ident t)
+        Definition show_ident_lvl (with_casts : bool) (with_all_casts : bool) {t} (idc : ident.ident t)
           : type.for_each_lhs_of_arrow (fun t => (Level.Level -> string) * ZRange.type.option.interp t)%type t -> (Level.Level -> string) * ZRange.type.base.option.interp (type.final_codomain t)
-          := match idc in ident.ident t return type.for_each_lhs_of_arrow (fun t => (Level.Level -> string) * ZRange.type.option.interp t)%type t -> (Level.Level -> string) * ZRange.type.base.option.interp (type.final_codomain t) with
+          := let with_casts := (with_casts && negb with_all_casts)%bool in
+             match idc in ident.ident t return type.for_each_lhs_of_arrow (fun t => (Level.Level -> string) * ZRange.type.option.interp t)%type t -> (Level.Level -> string) * ZRange.type.base.option.interp (type.final_codomain t) with
              | ident.Literal base.type.Z v => fun 'tt => (show_lvl_compact_Z v, ZRange.type.base.option.None)
              | ident.Literal t v => fun 'tt => (show_lvl v, ZRange.type.base.option.Some (t:=t) v)
              | ident.tt => fun _ => (fun _ => "()", tt)
@@ -630,8 +646,7 @@ Module Compilers.
              | ident.Z_gtb as idc
              | ident.Z_geb as idc
                => fun '(x, (y, tt)) => (show_lvl_binop idc (maybe_wrap_cast with_casts x) (maybe_wrap_cast with_casts y), ZRange.type.base.option.None)
-             | ident.pair _ _ as idc
-               => fun '((x, xr), ((y, yr), tt)) => (show_lvl_binop_no_space idc x y, ZRange.type.base.option.None)
+             | ident.pair _ _ as idc => fun '((x, xr), ((y, yr), tt)) => (show_lvl_binop_no_space idc x y, (xr, yr))
              | ident.fst _ _ as idc
                => fun '((x, xr), tt) => (show_lvl_postop idc x, fst xr)
              | ident.snd _ _ as idc
@@ -647,10 +662,22 @@ Module Compilers.
              | ident.List_nth_default _
                => fun '((d, dr), ((ls, lsr), ((i, ir), tt))) => (fun lvl => maybe_wrap_parens (Level.ltb lvl app_lvl) (show_lvl ls app_lvl ++ "[" ++ show_lvl i term_lvl ++ "]"), ZRange.type.base.option.None)
              | ident.Z_lnot_modulo => fun '((x, xr), ((m, mr), tt)) => (fun lvl => maybe_wrap_parens (Level.ltb lvl 75) ("~" ++ show_lvl x 75 ++ (if with_casts then " (mod " ++ show_lvl m term_lvl ++ ")" else "")), ZRange.type.base.option.None)
-             | ident.Z_cast
-             | ident.Z_cast2
-               => fun '((_, range), ((x, xr), tt)) => (x, range)
-             | ident.Build_zrange => fun '((x, xr), ((y, yr), tt)) => (neg_wrap_parens ("r[" ++ show_lvl x 60 ++ " ~> " ++ show_lvl y term_lvl), ZRange.type.base.option.None)
+             | ident.Z_cast as idc
+             | ident.Z_cast2 as idc
+               => fun '((srange, range), ((x, xr), tt))
+                  => let t := (fun t (idc : ident.ident (_ -> t -> _)) => t) _ idc in
+                     (* if we don't do the above, we pick up the wrong type in maybe_wrap_cast below *)
+                     (if with_all_casts && Option.is_None (ZRange.type.base.option.lift_Some range)
+                      then (fun _ => "(" ++ srange term_lvl ++ ")" ++ x 0)
+                      else maybe_wrap_cast (t:=t) with_all_casts (x, range),
+                       range)
+             | ident.Build_zrange
+               => fun '((x, xr), ((y, yr), tt))
+                  => (neg_wrap_parens ("r[" ++ show_lvl x 60 ++ " ~> " ++ show_lvl y term_lvl),
+                       match ZRange.ident.option.to_literal xr, ZRange.ident.option.to_literal yr with
+                       | Some l, Some h => Some r[l ~> h]
+                       | _, _ => (*ZRange.type.base.option.*)None
+                       end)
              | ident.comment _ as idc
              | ident.comment_no_keep _ as idc
              | ident.value_barrier as idc
@@ -799,45 +826,46 @@ Module Compilers.
                 end r).
         End helper.
 
-        Fixpoint show_expr_lines_gen (with_casts : bool) {var} (to_string : forall t, var t -> string) (of_string : forall t, string -> option (var t)) {t} (e : @API.expr var t) (args : type.for_each_lhs_of_arrow (fun t => (Level -> string) * ZRange.type.option.interp t)%type t) (idx : positive) {struct e} : (positive * (Level -> list string)) * ZRange.type.base.option.interp (type.final_codomain t)
-          := match e in expr.expr t return type.for_each_lhs_of_arrow (fun t => (Level -> string) * ZRange.type.option.interp t)%type t -> (positive * (Level -> list string)) * ZRange.type.base.option.interp (type.final_codomain t) with
+        Fixpoint show_expr_lines_gen (with_casts : bool) (with_all_casts : bool) {var} (to_string : forall t, var t -> string) (of_string : forall t, string -> option (var t)) {t} (e : @API.expr var t) (args : type.for_each_lhs_of_arrow (fun t => (Level -> string) * ZRange.type.option.interp t)%type t) (idx : positive) {struct e} : (positive * (Level -> list string)) * ZRange.type.base.option.interp (type.final_codomain t)
+          := let show_expr_lines_gen := @show_expr_lines_gen with_casts with_all_casts var to_string of_string in
+             match e in expr.expr t return type.for_each_lhs_of_arrow (fun t => (Level -> string) * ZRange.type.option.interp t)%type t -> (positive * (Level -> list string)) * ZRange.type.base.option.interp (type.final_codomain t) with
              | expr.Ident t idc
-               => fun args => let '(v, r) := @show_ident_lvl with_casts t idc args in
+               => fun args => let '(v, r) := @show_ident_lvl with_casts with_all_casts t idc args in
                               (idx, fun lvl => [v lvl], r)
              | expr.Var t v
                => fun args => (idx, fun lvl => [show_application with_casts (fun _ => to_string _ v) args lvl], ZRange.type.base.option.None)
              | expr.Abs s d f
                => fun args
-                  => show_eta_abs_cps of_string (fun t e args idx => let '(idx, v, r) := @show_expr_lines_gen with_casts var to_string of_string t e args idx in (idx, fun _ => v term_lvl, r)) with_casts idx f args
+                  => show_eta_abs_cps of_string (fun t e args idx => let '(idx, v, r) := @show_expr_lines_gen t e args idx in (idx, fun _ => v term_lvl, r)) with_casts idx f args
              | expr.App s d f x
                => fun args
-                  => let '(idx', x', xr) := show_eta_cps of_string (fun t e args idx => @show_expr_lines_gen with_casts var to_string of_string t e args idx) idx x in
+                  => let '(idx', x', xr) := show_eta_cps of_string (fun t e args idx => @show_expr_lines_gen t e args idx) idx x in
                      @show_expr_lines_gen
-                       with_casts var to_string of_string _ f
+                       _ f
                        (((fun lvl => String.concat String.NewLine (x' lvl)), xr),
-                        args)
+                         args)
                        idx
              | expr.LetIn A (type.base B) x f
                => fun 'tt
                   => let n := "x" ++ Decimal.Pos.to_string idx in
-                     let '(_, show_x, xr) := show_eta_cps of_string (fun t e args idx => @show_expr_lines_gen with_casts var to_string of_string t e args idx) idx x in
+                     let '(_, show_x, xr) := show_eta_cps of_string (fun t e args idx => @show_expr_lines_gen t e args idx) idx x in
                      let '(idx, show_f, fr)
-                         := match of_string A n with
-                            | Some n' => show_eta_cps of_string (fun t e args idx => @show_expr_lines_gen with_casts var to_string of_string t e args idx) (Pos.succ idx) (f n')
-                            | None => (idx, (fun _ => ["_"]), ZRange.type.option.None)
-                            end in
+                       := match of_string A n with
+                          | Some n' => show_eta_cps of_string (fun t e args idx => @show_expr_lines_gen t e args idx) (Pos.succ idx) (f n')
+                          | None => (idx, (fun _ => ["_"]), ZRange.type.option.None)
+                          end in
                      let '(ty_str, comment_ty_str, space_comment_ty_str)
-                         := match make_cast xr with
-                            | Some c => let ty_str := " : " ++ c in
-                                        let comment_ty_str := "(*" ++ ty_str ++ " *)" in
-                                        (ty_str, comment_ty_str, " " ++ comment_ty_str)
-                            | None => ("", "", "")
-                            end in
+                       := match make_cast xr with
+                          | Some c => let ty_str := " : " ++ c in
+                                      let comment_ty_str := "(*" ++ ty_str ++ " *)" in
+                                      (ty_str, comment_ty_str, " " ++ comment_ty_str)
+                          | None => ("", "", "")
+                          end in
                      let expr_let_line := "let " ++ n ++ " := " in
                      (idx,
-                      (fun lvl
-                       => match show_x term_lvl with
-                          | nil => [expr_let_line ++ "(* NOTHING‽ *)" ++ space_comment_ty_str ++ " in"]%string ++ show_f term_lvl
+                       (fun lvl
+                        => match show_x term_lvl with
+                           | nil => [expr_let_line ++ "(* NOTHING‽ *)" ++ space_comment_ty_str ++ " in"]%string ++ show_f term_lvl
                           | show_x::nil => [expr_let_line ++ show_x ++ "" ++ space_comment_ty_str ++ " in"]%string ++ show_f term_lvl
                           | show_x::rest
                             => ([expr_let_line ++ show_x]%string)
@@ -851,10 +879,10 @@ Module Compilers.
              | expr.LetIn A B x f
                => fun args
                   => let n := "x" ++ Decimal.Pos.to_string idx in
-                     let '(_, show_x, xr) := show_eta_cps of_string (fun t e args idx => @show_expr_lines_gen with_casts var to_string of_string t e args idx) idx x in
+                     let '(_, show_x, xr) := show_eta_cps of_string (fun t e args idx => @show_expr_lines_gen t e args idx) idx x in
                      let '(idx, show_f, fr)
                          := match of_string A n with
-                            | Some n' => show_eta_cps of_string (fun t e args idx => @show_expr_lines_gen with_casts var to_string of_string t e args idx) (Pos.succ idx) (f n')
+                            | Some n' => show_eta_cps of_string (fun t e args idx => @show_expr_lines_gen t e args idx) (Pos.succ idx) (f n')
                             | None => (idx, (fun _ => ["_"]), ZRange.type.option.None)
                             end in
                      let '(ty_str, comment_ty_str, space_comment_ty_str)
@@ -884,8 +912,8 @@ Module Compilers.
                              ++ [")"; show_application with_casts (fun _ => "") args (Level.prev app_lvl)])%list),
                       ZRange.type.base.option.None)
              end args.
-        Definition show_expr_lines (with_casts : bool) {t} (e : @API.expr (fun _ => string) t) (args : type.for_each_lhs_of_arrow (fun t => (Level -> string) * ZRange.type.option.interp t)%type t) (idx : positive) : (positive * (Level -> list string)) * ZRange.type.base.option.interp (type.final_codomain t)
-          := @show_expr_lines_gen with_casts (fun _ => string) (fun _ x => x) (fun _ x => Some x) t e args idx.
+        Definition show_expr_lines (with_casts : bool) (with_all_casts : bool) {t} (e : @API.expr (fun _ => string) t) (args : type.for_each_lhs_of_arrow (fun t => (Level -> string) * ZRange.type.option.interp t)%type t) (idx : positive) : (positive * (Level -> list string)) * ZRange.type.base.option.interp (type.final_codomain t)
+          := @show_expr_lines_gen with_casts with_all_casts (fun _ => string) (fun _ x => x) (fun _ x => Some x) t e args idx.
         Definition show_lvl_var_expr : forall {var t}, ShowLevel (@API.expr var t)
           := fix show_lvl_var_expr {var t} (e : @API.expr var t) : Level -> string
                := match e with
@@ -898,24 +926,25 @@ Module Compilers.
                   end%string.
         Definition show_var_expr {var t} : Show (@API.expr var t) := show_lvl_var_expr.
         Definition partially_show_expr {var t} : Show (@API.expr var t) := show_var_expr.
-        Local Notation default_with_casts := true.
         Section Show_gen.
-          Context {var : API.type -> Type}
+          Context {with_casts : PHOAS.with_casts}
+                  {with_all_casts : PHOAS.with_all_casts}
+                  {var : API.type -> Type}
                   (to_string : forall t, var t -> string)
                   (of_string : forall t, string -> option (var t)).
 
           Definition show_lines_expr_gen {t} : ShowLines (@API.expr var t)
-            := fun e => let '(_, v, _) := show_eta_cps of_string (fun t e args idx => @show_expr_lines_gen default_with_casts var to_string of_string t e args idx) 1%positive e in v (Level.prev term_lvl).
+            := fun e => let '(_, v, _) := show_eta_cps of_string (fun t e args idx => @show_expr_lines_gen with_casts with_all_casts var to_string of_string t e args idx) 1%positive e in v (Level.prev term_lvl).
           Definition show_expr_gen {t} : Show (@API.expr var t)
             := fun e => String.concat String.NewLine (show_lines_expr_gen e).
         End Show_gen.
-        Global Instance show_lines_expr {t} : ShowLines (@API.expr (fun _ => string) t)
-          := @show_lines_expr_gen (fun _ => string) (fun _ x => x) (fun _ x => Some x) t.
-        Global Instance show_lines_Expr {t} : ShowLines (@API.Expr t)
+        Global Instance show_lines_expr {with_casts : PHOAS.with_casts} {with_all_casts : PHOAS.with_all_casts} {t} : ShowLines (@API.expr (fun _ => string) t)
+          := @show_lines_expr_gen with_casts with_all_casts (fun _ => string) (fun _ x => x) (fun _ x => Some x) t.
+        Global Instance show_lines_Expr {with_casts : PHOAS.with_casts} {with_all_casts : PHOAS.with_all_casts} {t} : ShowLines (@API.Expr t)
           := fun e => show_lines (e _).
-        Global Instance show_expr {t} : Show (@API.expr (fun _ => string) t)
+        Global Instance show_expr {with_casts : PHOAS.with_casts} {with_all_casts : PHOAS.with_all_casts} {t} : Show (@API.expr (fun _ => string) t)
           := fun e => String.concat String.NewLine (show_lines e).
-        Global Instance show_Expr {t} : Show (@API.Expr t)
+        Global Instance show_Expr {with_casts : PHOAS.with_casts} {with_all_casts : PHOAS.with_all_casts} {t} : Show (@API.Expr t)
           := fun e => show (e _).
       End expr.
     End PHOAS.
