src/SlowPrimeSynthesisExamples.v
@@ -2866,13 +2866,13 @@ Module debugging_go_build.
       cbv [Language.Compilers.ToString.PHOAS.expr.show_eta_cps] in XX.
       cbn [Language.Compilers.ToString.PHOAS.expr.show_eta_abs_cps'] in XX.
       cbv [Language.Compilers.ToString.PHOAS.expr.get_eta_cps_args] in XX.
-      set (k := Language.Compilers.ToString.PHOAS.expr.show_expr_lines _ _ _ _) in (value of XX) at 1.
+      set (k := Language.Compilers.ToString.PHOAS.expr.show_expr_lines _ _ _ _ _) in (value of XX) at 1.
       vm_compute in k.
       subst k; cbv beta iota zeta in XX.
-      set (k := Language.Compilers.ToString.PHOAS.expr.show_expr_lines _ _ _ _) in (value of XX) at 1.
+      set (k := Language.Compilers.ToString.PHOAS.expr.show_expr_lines _ _ _ _ _) in (value of XX) at 1.
       vm_compute in k.
       subst k; cbv beta iota zeta in XX.
-      set (k := Language.Compilers.ToString.PHOAS.expr.show_expr_lines _ _ _ _) in (value of XX) at 1.
+      set (k := Language.Compilers.ToString.PHOAS.expr.show_expr_lines _ _ _ _ _) in (value of XX) at 1.
       vm_compute in k.
       subst k; cbv beta iota zeta in XX.
       set (k := Language.Compilers.ToString.PHOAS.ident.show_ident_lvl _ _ _) in (value of XX).
@@ -2987,13 +2987,13 @@ Module debugging_go_output.
       cbv [Language.Compilers.ToString.PHOAS.expr.show_eta_cps] in XX.
       cbn [Language.Compilers.ToString.PHOAS.expr.show_eta_abs_cps'] in XX.
       cbv [Language.Compilers.ToString.PHOAS.expr.get_eta_cps_args] in XX.
-      set (k := Language.Compilers.ToString.PHOAS.expr.show_expr_lines _ _ _ _) in (value of XX) at 1.
+      set (k := Language.Compilers.ToString.PHOAS.expr.show_expr_lines _ _ _ _ _) in (value of XX) at 1.
       vm_compute in k.
       subst k; cbv beta iota zeta in XX.
-      set (k := Language.Compilers.ToString.PHOAS.expr.show_expr_lines _ _ _ _) in (value of XX) at 1.
+      set (k := Language.Compilers.ToString.PHOAS.expr.show_expr_lines _ _ _ _ _) in (value of XX) at 1.
       vm_compute in k.
       subst k; cbv beta iota zeta in XX.
-      set (k := Language.Compilers.ToString.PHOAS.expr.show_expr_lines _ _ _ _) in (value of XX) at 1.
+      set (k := Language.Compilers.ToString.PHOAS.expr.show_expr_lines _ _ _ _ _) in (value of XX) at 1.
       vm_compute in k.
       subst k; cbv beta iota zeta in XX.
       set (k := Language.Compilers.ToString.PHOAS.ident.show_ident_lvl _ _ _) in (value of XX).
